make the implementation of `NetAddr` more meaningful

Structures/Address.v
@@ -1,5 +1,5 @@
 From Coq Require Import Lia List.
-From Bythos.Utils Require Export Tactics.
+From Bythos.Utils Require Export Tactics ListFacts Misc.
 
 Module Type NetAddr.
 
@@ -8,6 +8,8 @@ Parameter Address_eqdec : forall (a1 a2 : Address), {a1 = a2} + {a1 <> a2}.
 Parameter Address_inhabitant : Address.
 
 (* restricting Address to be a finite type should be enough *)
+(* the Finite typeclass defined in stdpp could be used, but since the development mostly
+    uses the definitions in the Coq standard library (e.g., List.NoDup), so did not do that *)
 Parameter valid_nodes : list Address.
 Axiom valid_nodes_NoDup : NoDup valid_nodes.
 Axiom Address_is_finite : forall a : Address, In a valid_nodes.
@@ -26,7 +28,7 @@ Import finite fin.
 
 Definition Address := fin 5.
 Definition Address_eqdec := @fin_dec 5.
-Definition Address_inhabitant : Fin.t 5 := Fin.F1.
+Definition Address_inhabitant : Address := Fin.F1.
 
 Definition valid_nodes := enum (fin 5).
 Lemma valid_nodes_NoDup : List.NoDup valid_nodes.
@@ -37,3 +39,254 @@ Proof. setoid_rewrite <- elem_of_list_In. exact elem_of_enum. Qed.
 Definition N := length valid_nodes.
 
 End AddrAsFiniteType.
+
+(* another definition, in the subtype-like form *)
+
+Module AddrAsFiniteType2 <: NetAddr.
+
+Module IsTrue.
+
+(* using "b = true" should also work, but here we want to avoid considering equalities of identity proofs *)
+Definition isTrue (b : bool) : Prop := if b then True else False.
+Fact isTrue_true_iff b : isTrue b <-> b = true.
+Proof. destruct b; unfold isTrue; intuition. Qed.
+Fact isTrue_same_eq b (H1 H2 : isTrue b) : H1 = H2.
+Proof. destruct b; simpl in *; try contradiction. now destruct H1, H2. Qed.
+Fact isTrue_andb b1 b2 : isTrue (b1 && b2) <-> isTrue b1 /\ isTrue b2.
+Proof. destruct b1, b2; intuition; try exact I. Qed. 
+
+End IsTrue.
+
+Module AnotherFiniteType.
+
+Export IsTrue.
+
+(* this is essentially a special case of { x | P x }, where P has proof irrelevance
+    and only a finite number of elements satisfy P (so this becomes a finite type) *)
+(* a very close formalization can be found in mathcomp (the ordinal type), 
+    which depends on too many other definitions though *)
+Inductive fin_nat (n : nat) : Set := FT (m : nat) (H : isTrue (Nat.ltb m n)).
+Definition fin_nat_eqdec [n : nat] (m1 m2 : fin_nat n) : {m1 = m2} + {m1 <> m2}.
+  destruct m1 as [ m1 H1 ], m2 as [ m2 H2 ].
+  destruct (PeanoNat.Nat.eq_dec m1 m2) as [ -> | Hneq ].
+  - left. f_equal. apply isTrue_same_eq.
+  - right. intros [=->]. contradiction.
+Defined.
+Definition fin_nat_rank [n : nat] (a : fin_nat n) : nat :=
+  match a with FT _ m _ => S m end.
+Fact fin_nat_cmp n (m1 m2 : fin_nat n) : m1 = m2 <-> fin_nat_rank m1 = fin_nat_rank m2.
+Proof. 
+  split; intros; try congruence.
+  (* seems not very convenient to reason about fin_nat_eqdec *)
+  (*
+  destruct (fin_nat_eqdec m1 m2) eqn:E; try congruence. unfold fin_nat_eqdec in E. 
+  destruct m1 as [ m1 ? ], m2 as [ m2 ? ]. simpl in H. 
+  destruct (PeanoNat.Nat.eq_dec m1 m2); simpl in E; try discriminate. 
+  *)
+  (* using the same logic as fin_nat_eqdec *)
+  destruct m1 as [ m1 ? ], m2 as [ m2 ? ]. simpl in H. injection H as ->. f_equal. apply isTrue_same_eq.
+Qed.
+
+Fact le_left_minus_1 n m : S n <= m -> n <= m. Proof. lia. Qed.
+Fact le_left_minus_1' n m : isTrue (Nat.leb (S n) m) -> isTrue (Nat.leb n m). 
+Proof. rewrite !isTrue_true_iff, !PeanoNat.Nat.leb_le. lia. Qed.
+(* the following requires some tweak to ensure proof irrelevance *)
+(*
+Fixpoint fin_nat_enum_aux (n m : nat) (H : m <= n) : list (fin_nat n).
+  destruct m as [ | m' ].
+  - exact nil.
+  - exact (FT n m' (proj2 (isTrue_true_iff _) (proj2 (PeanoNat.Nat.ltb_lt _ _) H)) ::
+      fin_nat_enum_aux n m' (le_left_minus_1 _ _ H)).
+Defined.
+*)
+Fixpoint fin_nat_enum_aux (n m : nat) (H : isTrue (Nat.leb m n)) {struct m} : list (fin_nat n).
+  destruct m as [ | m' ].
+  - exact nil.
+  - exact (FT n m' H :: fin_nat_enum_aux n m' (le_left_minus_1' _ _ H)). 
+Defined.
+Definition fin_nat_enum (n : nat) : list (fin_nat n) :=
+  fin_nat_enum_aux n n (proj2 (isTrue_true_iff _) (PeanoNat.Nat.leb_refl n)).
+Fact fin_nat_enum_aux_incl n m1 m2 (H : m1 <= m2) H1 H2 : incl (fin_nat_enum_aux n m1 H1) (fin_nat_enum_aux n m2 H2).
+Proof.
+  revert n H1 H2. induction H as [ | m2 H IH ]; intros.
+  - rewrite (isTrue_same_eq _ H1 H2). hnf; auto.
+  - simpl. hnf. intros ? Hin. unshelve eapply IH in Hin; auto.
+    1: now apply le_left_minus_1'.
+    simpl. auto.
+Qed.
+Fact fin_nat_enum_complete n : forall a : fin_nat n, In a (fin_nat_enum n).
+Proof.
+  intros [ m H ].
+  assert (In (FT n m H) (fin_nat_enum_aux n (S m) H)) as H0 by (simpl; auto).
+  revert H0. now apply fin_nat_enum_aux_incl, PeanoNat.Nat.ltb_lt, isTrue_true_iff.
+Qed.
+Fact fin_nat_enum_aux_NoDup n m H : NoDup (fin_nat_enum_aux n m H).
+Proof.
+  match goal with |- ?G => enough (G /\ list_max (map (@fin_nat_rank n) (fin_nat_enum_aux n m H)) = m); try tauto end.
+  revert H. induction m as [ | m IH ]; intros; simpl.
+  - split; constructor.
+  - split.
+    + specialize (IH (le_left_minus_1' m n H)). destruct IH as (Ha & Hb). 
+      constructor; auto. 
+      intros Hin. epose proof (list_max_le _ _) as H0. rewrite Hb in H0. apply proj1 in H0. specialize (H0 (le_n _)).
+      rewrite Forall_forall in H0. specialize (H0 _ (in_map _ _ _ Hin)). simpl in H0. lia.
+    + rewrite (proj2 (IH _)). lia.
+Qed.
+Corollary fin_nat_enum_NoDup n : NoDup (fin_nat_enum n). 
+Proof. apply fin_nat_enum_aux_NoDup. Qed.
+
+Global Instance fin_nat_decision n : base.EqDecision (fin_nat n) := @fin_nat_eqdec n.
+Global Program Instance fin_nat_finite n : finite.Finite (fin_nat n) :=
+  {| finite.enum := fin_nat_enum n |}.
+Next Obligation. intros n. apply base.NoDup_ListNoDup, fin_nat_enum_NoDup. Qed.
+Next Obligation. intros n a. apply base.elem_of_list_In, fin_nat_enum_complete. Qed.
+
+End AnotherFiniteType.
+
+Import AnotherFiniteType.
+
+(* after extraction, it will become just natural number pairs *)
+Definition Address := prod (fin_nat 5) (fin_nat 5).
+Definition Address_eqdec := prod_eq_dec (@fin_nat_eqdec 5) (@fin_nat_eqdec 5).
+Definition Address_inhabitant : Address := (FT 5 0 I, FT 5 0 I).
+
+(* implicitly involving the instance of building Finite for products *)
+Definition valid_nodes : list Address := finite.enum Address.
+Lemma valid_nodes_NoDup : List.NoDup valid_nodes.
+Proof. apply base.NoDup_ListNoDup, finite.NoDup_enum. Qed.
+Lemma Address_is_finite : forall a : Address, In a valid_nodes.
+Proof. intros ?. apply base.elem_of_list_In, finite.elem_of_enum. Qed.
+
+Definition N := length valid_nodes.
+
+End AddrAsFiniteType2.
+
+(* the module above seems not to be the best for extraction work ... 
+    it involves some constructions in stdpp (e.g., Finite), which may result in the occurrences of 
+    weird things like Obj.magic *)
+
+(* defining the inductive type outside the module would not result in extracting its induction principles, 
+    which also involve Obj.somethings *)
+
+Inductive fin_mem {A : Type} (eqdec : forall a1 a2 : A, {a1 = a2} + {a1 <> a2}) (dom : list A) : Type :=
+  FM (a : A) (H : AddrAsFiniteType2.IsTrue.isTrue (ssrbool.is_left (in_dec eqdec a dom))).
+
+Module MembershipFiniteType.
+
+Export AddrAsFiniteType2.IsTrue.
+
+(* again, a special case of { x | P x } *)
+(* after extraction, the inductive type parameters will be cleared ... *)
+
+Section Main.
+
+  Context {A : Type} [eqdec : forall a1 a2 : A, {a1 = a2} + {a1 <> a2}] [dom : list A].
+
+  Local Notation fin_mem := (fin_mem eqdec dom).
+
+  Definition fin_mem_eqdec (m1 m2 : fin_mem) : {m1 = m2} + {m1 <> m2}.
+    destruct m1 as [ m1 H1 ], m2 as [ m2 H2 ].
+    destruct (eqdec m1 m2) as [ -> | Hneq ].
+    - left. f_equal. apply isTrue_same_eq.
+    - right. intros [=->]. contradiction.
+  Defined.
+
+  Definition fin_mem_body (m : fin_mem) := match m with FM _ _ a _ => a end.
+  Fact fin_mem_in a l : In a l <-> In (fin_mem_body a) (map fin_mem_body l).
+  Proof.
+    split; intros H; auto using in_map.
+    induction l as [ | a' l IH ]; simpl in *; auto. destruct H; try tauto.
+    destruct a as [ a H0 ], a' as [ a' H0' ]. simpl in H. 
+    left. revert H0'. rewrite H. (* ! *) intros ?. f_equal. apply isTrue_same_eq.
+  Qed.
+  (*
+  Definition fin_mem_lift_single (a : A.t) : list fin_mem :=
+    (if in_dec eqdec a A.elements as s0
+        return ((isTrue (ssrbool.is_left s0) -> fin_mem) -> list fin_mem)
+      then fun f0 : True -> fin_mem => f0 I :: nil
+      else fun _ : False -> fin_mem => nil) (FM a).
+    (* pose proof (FM a) as f.
+    destruct (in_dec eqdec a A.elements).
+    - exact (f I :: nil).
+    - exact nil.
+  Defined. *)
+  Fixpoint fin_mem_lift (l : list A.t) : list fin_mem :=
+    match l with
+    | nil => nil
+    | a :: l' => fin_mem_lift_single a ++ fin_mem_lift l'
+    end.
+  Fact fin_mem_lift_peel l (H : incl l A.elements) : map fin_mem_body (fin_mem_lift l) = l.
+  Proof.
+    induction l as [ | a l IH ]; try reflexivity.
+    simpl. pose proof (H _ (or_introl eq_refl)) as H0. specialize (IH (fun a H' => H a (or_intror H'))).
+    rewrite map_app, IH. change (a :: l) with ((a :: nil) ++ l). f_equal. clear H IH.
+    unfold fin_mem_lift_single.
+    (* emm *)
+  Abort.
+  *)
+  (* things are slightly more complicated without carrying a proof *)
+  Fixpoint fin_mem_lift (l : list A) (H : isTrue (forallb (fun a => ssrbool.is_left (in_dec eqdec a dom)) l)) {struct l} : list fin_mem.
+    destruct l as [ | a l' ].
+    - exact nil.
+    - simpl in H. apply (proj1 (isTrue_andb _ _)) in H. destruct H as (H1 & H2).
+      exact (FM _ _ a H1 :: fin_mem_lift _ H2).
+  Defined.
+  Fact fin_mem_lift_qualified l (H : incl l dom) : isTrue (forallb (fun a => ssrbool.is_left (in_dec eqdec a dom)) l).
+  Proof.
+    induction l as [ | a l' IH ]; simpl; auto.
+    rewrite isTrue_andb. pose proof (H _ (or_introl eq_refl)) as H0. specialize (IH (fun a H' => H a (or_intror H'))).
+    split; auto. unfold ssrbool.is_left. rewrite (proj2 (sumbool_is_left _)); hnf; auto.
+  Qed.
+  Fact fin_mem_lift_peel l H : map fin_mem_body (fin_mem_lift l H) = l.
+  Proof.
+    induction l as [ | a l' IH ]; simpl; auto.
+    destruct (proj1 _ _). (* ... *) simpl. f_equal. now rewrite IH.
+  Qed.
+  Fact fin_mem_lift_NoDup l H (Hnodup : List.NoDup l) : List.NoDup (fin_mem_lift l H).
+  Proof.
+    induction l as [ | a l IH ]; simpl; try solve [ constructor ].
+    apply NoDup_cons_iff in Hnodup. destruct Hnodup as (Hnotin & Hnodup).
+    destruct (proj1 _ _). (* ... *) constructor. 2: apply IH; auto.
+    rewrite fin_mem_in. simpl. now rewrite fin_mem_lift_peel.
+  Qed.
+
+End Main.
+
+End MembershipFiniteType.
+
+Module Type JustAList.
+
+Parameter t : Set.
+Parameter t_eqdec : forall a b : t, {a = b} + {a <> b}.
+
+Parameter elements : list t.
+Parameter elements_not_empty : elements <> nil.
+Parameter elements_NoDup : List.NoDup elements.
+
+End JustAList.
+
+Module AddrAsFiniteType3 (A : JustAList) <: NetAddr.
+
+Import MembershipFiniteType.
+
+Local Notation fin_mem := (fin_mem A.t_eqdec A.elements).
+
+Definition Address := fin_mem.
+Definition Address_eqdec := @fin_mem_eqdec _ A.t_eqdec A.elements.
+Definition Address_inhabitant : Address.
+  pose proof A.elements_not_empty as H. destruct A.elements as [ | a ? ] eqn:E; try contradiction.
+  eapply FM with (a:=a). unfold ssrbool.is_left. rewrite (proj2 (sumbool_is_left _)); hnf; auto. rewrite E. apply (or_introl eq_refl).
+Qed.
+
+Definition valid_nodes : list Address := fin_mem_lift A.elements (fin_mem_lift_qualified _ (incl_refl _)).
+Lemma valid_nodes_NoDup : List.NoDup valid_nodes.
+Proof. apply fin_mem_lift_NoDup, A.elements_NoDup. Qed.
+Lemma Address_is_finite : forall a : Address, In a valid_nodes.
+Proof. 
+  intros [ ? H ]. pose proof H as H0%isTrue_true_iff%sumbool_is_left. 
+  apply fin_mem_in. simpl. unfold valid_nodes. now rewrite fin_mem_lift_peel.
+Qed.
+
+Definition N := length valid_nodes.
+
+End AddrAsFiniteType3.
